Stuck while trying to implement the running example.

io/RunningExample.fst
@@ -1,6 +1,9 @@
 module RunningExample
 
-open Compiler.Languages
+open FStar.Ghost
+open FStar.List.Tot.Base
+
+open Compiler.Model
 
 assume val valid_http_response : string -> bool
 assume val valid_http_request : string -> bool
@@ -11,31 +14,58 @@ let did_not_respond h =
   | EWrite _ _ _ :: _ -> false
   | _ -> true
 
-open FStar.List.Tot.Base
-
 val handler_only_openfiles_reads_client_acc : trace -> list file_descr -> bool
-let rec handler_only_openfiles_reads_client_acc lt open_descr =
+let rec handler_only_openfiles_reads_client_acc lt open_descrs =
   match lt with
   | [] -> true
-  | EWrite true _ _ :: tl -> handler_only_openfiles_reads_client_acc tl open_descr
+  | EOpenfile true  _ _ :: tl -> handler_only_openfiles_reads_client_acc tl open_descrs
+  | ERead true  _ _ :: tl -> handler_only_openfiles_reads_client_acc tl open_descrs
+  | EWrite true _ _ :: tl -> handler_only_openfiles_reads_client_acc tl open_descrs
+  | EClose true  _ _ :: tl -> handler_only_openfiles_reads_client_acc tl open_descrs
   | EOpenfile false fnm res :: tl -> 
     if fnm = "/temp" then begin
       match res with
-      | Inl fd -> handler_only_openfiles_reads_client_acc tl (fd::open_descr)
-      | Inr err -> handler_only_openfiles_reads_client_acc tl open_descr
+      | Inl fd -> handler_only_openfiles_reads_client_acc tl (fd::open_descrs)
+      | Inr err -> handler_only_openfiles_reads_client_acc tl open_descrs
     end else false
   | ERead false fd _ :: tl -> 
-    if fd `mem` open_descr then handler_only_openfiles_reads_client_acc tl open_descr
+    if fd `mem` open_descrs then handler_only_openfiles_reads_client_acc tl open_descrs
     else false
+  | EWrite false _ _ :: tl -> false
   | EClose false fd _ :: tl -> 
-    if fd `mem` open_descr then handler_only_openfiles_reads_client_acc tl (filter (fun fd' -> fd <> fd') open_descr)
+    if fd `mem` open_descrs then handler_only_openfiles_reads_client_acc tl (filter (fun fd' -> fd <> fd') open_descrs)
     else false
-  | _ :: tl -> false
 
 val handler_only_openfiles_reads_client : trace -> bool
 let handler_only_openfiles_reads_client lt =
   handler_only_openfiles_reads_client_acc lt []
-  
+
+let rec is_opened_by_untrusted (h:trace) (fd:file_descr) : bool =
+  match h with
+  | [] -> false
+  | EOpenfile false _ (Inl fd') :: tl -> begin
+    if fd = fd' then true
+    else is_opened_by_untrusted tl fd
+  end
+  | EClose _ fd' (Inl ()) :: tl -> if fd = fd' then false
+                             else is_opened_by_untrusted tl fd
+  | _ :: tl -> is_opened_by_untrusted tl fd
+
+val pi : monitorable_prop
+let pi h cmd arg =
+  match cmd with
+  | Openfile -> 
+    if arg = "/temp" then true else false
+  | Read -> is_opened_by_untrusted h arg
+  | Close -> is_opened_by_untrusted h arg
+  | _ -> false
+
+let rec lemma1 (lt h:trace) : Lemma (requires (enforced_locally pi h lt)) (ensures (handler_only_openfiles_reads_client lt)) =
+  match lt with
+  | [] -> ()
+  | e::tl -> admit ()//  lemma1 tl (e::h)
+
+
 val wrote_at_least_once_to : file_descr -> trace -> bool
 let rec wrote_at_least_once_to client lt =
   match lt with
@@ -52,15 +82,79 @@ type request_handler =
                                                    (ensures (fun _ _ lt -> exists r. lt == [EWrite true (client,msg) r] /\
                                                                          wrote_at_least_once_to client lt)))) ->
   IIO (resexn unit) IOActions (requires (fun h -> valid_http_request req /\ did_not_respond h))
-                              (ensures (fun _ _ lt -> handler_only_openfiles_reads_client lt /\
+                              (ensures (fun h _ lt -> enforced_locally pi h lt /\
                                                     wrote_at_least_once_to client lt))
 
 assume val req_res : req:string{valid_http_request req} -> res:string{valid_http_response res}
-
-open FStar.Tactics
 
 val source_handler : request_handler
 let source_handler client req send =
   let res = req_res req in
   let _ = send res in 
+  Inl ()
+
+val every_request_gets_a_response_acc : trace -> list file_descr -> Type0
+let rec every_request_gets_a_response_acc lt read_descrs =
+  match lt with
+  | [] -> read_descrs == []
+  | ERead true fd (Inl _)::tl -> every_request_gets_a_response_acc tl (fd::read_descrs)
+  | EWrite true (fd,_) _::tl -> every_request_gets_a_response_acc tl (filter (fun fd' -> fd <> fd') read_descrs)
+  | _::tl -> every_request_gets_a_response_acc tl read_descrs
+
+val every_request_gets_a_response : trace -> Type0
+let every_request_gets_a_response lt =
+  every_request_gets_a_response_acc lt []
+
+assume val get_req : file_descr -> option (req:string{valid_http_request req})
+assume val sendError : int -> fd:file_descr -> IIO unit IOActions
+ (fun _ -> True) (fun _ _ lt -> exists (msg:string) r. lt == [EWrite true (fd, msg) r])
+
+open FStar.Tactics
+
+(* Stuck: enforcing the access policy on the context, gives as a 
+   trace property that talks about the events produced by the context.
+   However, one also has to talk about the events produced by the program
+   inside the context. 
+
+   Otherwise, we can not prove every_request_gets_a_response post-condition,
+   because theoretically the partial program can produce events 
+   inside the context that violate the condition.
+   
+   One can manually adnotate the post-condition of the handler to say 
+   that it includes only writes of the partial program, but then
+   we cannot enforce it with the access policy or higher-order contracts.
+   Can we find some kind of property that makes it safe to
+   ``forget"?
+
+   Another strategy would be to find a different post-condition for
+   the webserver :D.
+*)
+
+let webserver (handler:request_handler) :
+  IIO (resexn unit) IOActions
+    (requires (fun h -> True))
+    (ensures (fun _ _ lt -> every_request_gets_a_response lt)) by
+  (explode (); bump_nth 49; 
+    rewrite_eqs_from_context (); dump "H") =
+  let client = static_cmd true Openfile "test.txt" in
+  match client with | Inr err -> Inr err | Inl client -> begin
+    match get_req client with
+    | Some req -> handler client req (fun res -> static_cmd true Write (client,res))
+    | None -> sendError 400 client;
+    static_cmd true Close client
+  end
+
+
+type tgt_handler =
+  (fl:erased tflag) ->
+  (pi:erased monitorable_prop) ->
+  (io_acts:acts fl pi false) ->
+  (client:file_descr) ->
+  (req:string) ->
+  (send:(msg:string -> IIOpi (resexn unit) fl pi)) ->
+  IIOpi (resexn unit) fl pi
+
+val target_handler : tgt_handler
+let target_handler fl pi io_acts client req send =
+  let _ = send req in 
   Inl ()
